concurrent two-inode API on top of concurrent predicate-lifting log

src/Examples/Logging2/AllocAPI.v
@@ -47,3 +47,50 @@ Module Alloc.
        initP := fun s => s = ∅ |}.
 
 End Alloc.
+
+Module Inode.
+
+  Inductive Op : Type -> Type :=
+  | Read (i : nat) : Op (nat*nat)
+  | Write2 (i : nat) (v0 v1 : nat) : Op unit.
+
+  Definition State : Type := ((nat*nat) * (nat*nat)).
+
+  Definition dynamics : Dynamics Op State :=
+    {| step T (op: Op T) :=
+         match op with
+         | Read 0 =>
+            reads (fun s => fst s)
+         | Read 1 =>
+            reads (fun s => snd s)
+         | Read _ => pure (0, 0)
+         | Write2 0 v0 v1 =>
+            puts (fun s => ((v0, v1), snd s))
+         | Write2 1 v0 v1 =>
+            puts (fun s => (fst s, (v0, v1)))
+         | Write2 _ _ _ => pure tt
+         end;
+       crash_step := pure tt;
+       finish_step := pure tt;
+    |}.
+
+  Lemma crash_total_ok (s: State):
+    exists s', dynamics.(crash_step) s (Val s' tt).
+  Proof. eexists; econstructor. Qed.
+
+  Lemma crash_non_err_ok (s: State) ret:
+    dynamics.(crash_step) s ret -> ret ≠ Err.
+  Proof. inversion 1; congruence. Qed.
+
+  Definition l : Layer Op :=
+    {| Layer.OpState := State;
+       sem := dynamics;
+       trace_proj := fun _ => nil;
+       crash_preserves_trace := fun _ _ _ => eq_refl;
+       crash_total := crash_total_ok;
+       finish_total := crash_total_ok;
+       crash_non_err := crash_non_err_ok;
+       finish_non_err := crash_non_err_ok;
+       initP := fun s => s = ((0,0),(0,0)) |}.
+
+End Inode.
